progs/conclib.v
@@ -1,0 +1,406 @@
+Require Export msl.predicates_sl.
+Require Import concurrency.semax_conc.
+Require Import floyd.proofauto.
+
+Lemma precise_sepcon : forall (P Q : mpred) (HP : precise P) (HQ : precise Q), precise (P * Q).
+Proof.
+  unfold precise; intros ??????? (l1 & r1 & Hjoin1 & HP1 & HQ1) (l2 & r2 & Hjoin2 & HP2 & HQ2)
+    Hsub1 Hsub2.
+  specialize (HP w _ _ HP1 HP2); specialize (HQ w _ _ HQ1 HQ2).
+  rewrite HP, HQ in Hjoin1.
+  eapply sepalg.join_eq; eauto.
+  - apply sepalg.join_sub_trans with (b := w1); auto.
+    eapply sepalg.join_join_sub'; eauto.
+  - apply sepalg.join_sub_trans with (b := w2); auto.
+    eapply sepalg.join_join_sub'; eauto.
+  - apply sepalg.join_sub_trans with (b := w1); auto.
+    eapply sepalg.join_join_sub; eauto.
+  - apply sepalg.join_sub_trans with (b := w2); auto.
+    eapply sepalg.join_join_sub; eauto.
+Qed.
+
+Lemma precise_andp1 : forall P Q (HP : precise P), precise (P && Q).
+Proof.
+  intros ?????? (? & ?) (? & ?) ??; eauto.
+Qed.
+
+Lemma precise_andp2 : forall P Q (HQ : precise Q), precise (P && Q).
+Proof.
+  intros ?????? (? & ?) (? & ?) ??; eauto.
+Qed.
+
+Lemma ex_address_mapsto_precise: forall ch rsh sh l,
+  precise (EX v : val, res_predicates.address_mapsto ch v rsh sh l).
+Proof.
+  intros.
+  eapply derives_precise, res_predicates.VALspec_range_precise.
+  repeat intro.
+  destruct H.
+  eapply res_predicates.address_mapsto_VALspec_range; eauto.
+Qed.
+
+Lemma mapsto_undef_precise : forall sh t b o (Hsh : readable_share sh)
+  (Hval : type_is_by_value t = true) (Hvol : type_is_volatile t = false),
+  precise (mapsto sh t (Vptr b o) Vundef).
+Proof.
+  intros; unfold mapsto.
+  destruct (access_mode_by_value _ Hval) as (? & Heq); rewrite Heq, Hvol.
+  destruct (readable_share_dec _); [|contradiction].
+  pose proof (tc_val_Vundef t).
+  intros ??? [(? & _) | (_ & HP1)] [(? & _) | (_ & HP2)]; normalize.
+  eapply ex_address_mapsto_precise; eauto.
+Qed.
+
+Lemma lock_inv_precise : forall v sh R, predicates_sl.precise (lock_inv sh v R).
+Proof.
+  repeat intro.
+  destruct H as (b & o & ? & Hlock).
+  admit.
+Admitted.
+
+Lemma lock_inv_positive : forall v sh R,
+  positive_mpred (lock_inv v sh R).
+Proof.
+  admit.
+Admitted.
+
+Lemma selflock_precise : forall R sh v, predicates_sl.precise R ->
+  predicates_sl.precise (selflock R v sh).
+Proof.
+  intros.
+  rewrite selflock_eq.
+  apply precise_sepcon; auto.
+  apply lock_inv_precise.
+Qed.
+
+Lemma positive_sepcon1 : forall P Q (HP : positive_mpred P),
+  positive_mpred (P * Q).
+Proof.
+  repeat intro.
+  destruct H as (? & ? & ? & HP1 & ?).
+  specialize (HP _ HP1).
+  destruct HP as (l & sh & rsh & k & p & HP); exists l, sh, rsh, k, p.
+  admit.
+Admitted.
+
+Lemma selflock_positive : forall R sh v, positive_mpred R ->
+  positive_mpred (selflock R v sh).
+Proof.
+  intros.
+  rewrite selflock_eq.
+  apply positive_sepcon1; auto.
+Qed.
+
+Lemma later_positive : forall P, positive_mpred P -> positive_mpred (|> P)%logic.
+Proof.
+  admit.
+Admitted.
+
+Lemma semax_fun_id'' id f Espec {cs} Delta P Q R Post c :
+  (var_types Delta) ! id = None ->
+  (glob_specs Delta) ! id = Some f ->
+  (glob_types Delta) ! id = Some (type_of_funspec f) ->
+  @semax cs Espec Delta
+    (EX v : val, PROPx P
+      (LOCALx (gvar id v :: Q)
+      (SEPx ((func_ptr' f v) :: R)))) c Post ->
+  @semax cs Espec Delta (PROPx P (LOCALx Q (SEPx R))) c Post.
+Proof.
+intros V G GS SA.
+apply (semax_fun_id id f Delta); auto.
+eapply semax_pre_post; try apply SA; [ clear SA |
+  intros; simpl; unfold local, lift1; entailer! ].
+go_lowerx.
+apply exp_right with (eval_var id (type_of_funspec f) rho).
+entailer.
+apply andp_right.
+- (* about gvar *)
+  apply prop_right.
+  unfold gvar_denote, eval_var, Map.get.
+  destruct H as (_ & _ & DG & DS).
+  destruct (DS id _ GS) as [-> | (t & E)]; [ | congruence].
+  destruct (DG id _ GS) as (? & -> & ?); auto.
+- (* about func_ptr/func_ptr' *)
+  unfold func_ptr'.
+  rewrite <- andp_left_corable, andp_comm; auto.
+  apply corable_func_ptr.
+Qed.
+
+Ltac get_global_function'' _f :=
+eapply (semax_fun_id'' _f); try reflexivity.
+
+Lemma lock_inv_join : forall sh1 sh2 sh v R (Hjoin : sepalg.join sh1 sh2 sh),
+  lock_inv sh1 v R * lock_inv sh2 v R = lock_inv sh v R.
+Proof.
+  admit.
+Admitted.
+
+Lemma split_readable_share sh :
+  readable_share sh ->
+  exists sh1, exists sh2,
+    readable_share sh1 /\
+    readable_share sh2 /\
+    sepalg.join sh1 sh2 sh.
+Admitted.
+
+Lemma split_Ews :
+  exists sh1, exists sh2,
+    readable_share sh1 /\
+    readable_share sh2 /\
+    sepalg.join sh1 sh2 Ews.
+Proof.
+  apply split_readable_share; auto.
+Qed.
+
+Lemma emp_almost_empty : forall phi, predicates_hered.app_pred emp phi -> juicy_machine.almost_empty phi.
+Proof.
+  repeat intro; subst.
+(*  Check compcert_rmaps.RML.resource_at_join.*)
+  admit.
+Admitted.
+
+Lemma prop_almost_empty : forall P phi, predicates_hered.app_pred (prop P) phi -> juicy_machine.almost_empty phi.
+Proof.
+  admit.
+Admitted.
+
+Lemma lock_inv_almost_empty : forall sh v R phi, predicates_hered.app_pred (lock_inv sh v R) phi ->
+  juicy_machine.almost_empty phi.
+Proof.
+  admit.
+Admitted.
+
+Lemma almost_empty_join : forall phi1 phi2 phi
+  (Hphi1 : juicy_machine.almost_empty phi1)
+  (Hphi2 : juicy_machine.almost_empty phi2)
+  (Hjoin : sepalg.join phi1 phi2 phi),
+  juicy_machine.almost_empty phi.
+Proof.
+  repeat intro.
+  specialize (Hphi1 loc sh psh k P); specialize (Hphi2 loc sh psh k P).
+  pose proof (compcert_rmaps.RML.resource_at_join _ _ _ loc Hjoin) as Hsum.
+  rewrite H in Hsum.
+(*  SearchAbout sepalg.join compcert_rmaps.RML.R.YES.*)
+  admit.
+Admitted.
+
+Lemma data_at_precise : forall {cs} b o,
+  precise (@data_at_ cs Ews (tarray tint 1) (Vptr b o)).
+Proof.
+  intros; unfold data_at_, field_at_, field_at, at_offset; simpl.
+  apply precise_andp2.
+  rewrite data_at_rec_eq; unfold withspacer, at_offset; simpl.
+  unfold array_pred, aggregate_pred.array_pred; simpl.
+  unfold Zlength, Znth; simpl.
+  apply precise_andp2.
+  rewrite data_at_rec_eq; simpl.
+  apply precise_sepcon; [apply mapsto_undef_precise | apply precise_emp]; auto.
+Qed.
+
+Lemma cond_var_precise : forall {cs} sh b o, readable_share sh ->
+  precise (@cond_var cs sh (Vptr b o)).
+Proof.
+  intros; unfold cond_var, data_at_, field_at_, field_at, at_offset; simpl.
+  apply precise_andp2.
+  rewrite data_at_rec_eq; simpl.
+  apply mapsto_undef_precise; auto.
+Qed.
+
+Lemma positive_sepcon2 : forall P Q (HQ : positive_mpred Q),
+  positive_mpred (P * Q).
+Proof.
+  repeat intro.
+  destruct H as (? & ? & ? & ? & HQ1).
+  specialize (HQ _ HQ1).
+  destruct HQ as (l & sh & rsh & k & p & HQ); exists l, sh, rsh, k, p.
+  admit.
+Admitted.
+
+Lemma lock_inv_isptr : forall sh v R, lock_inv sh v R = !!isptr v && lock_inv sh v R.
+Proof.
+  intros.
+  eapply local_facts_isptr with (P := fun v => lock_inv sh v R); eauto.
+  unfold lock_inv; Intros b o.
+  subst; simpl; entailer.
+Qed.
+
+Lemma cond_var_isptr : forall {cs} sh v, @cond_var cs sh v = !! isptr v && cond_var sh v.
+Proof.
+  intros; apply data_at__isptr.
+Qed.
+
+Lemma cond_var_almost_empty : forall {cs} sh v phi, predicates_hered.app_pred (@cond_var cs sh v) phi ->
+  juicy_machine.almost_empty phi.
+Proof.
+  admit.
+Admitted.
+
+Lemma cond_var_join : forall {cs} sh1 sh2 sh v (Hjoin : sepalg.join sh1 sh2 sh),
+  @cond_var cs sh1 v * cond_var sh2 v = cond_var sh v.
+Proof.
+  intros; unfold cond_var; apply data_at__share_join; auto.
+Qed.
+
+Definition complete MAX l := l ++ repeat (Vint (Int.repr 0)) (MAX - length l).
+
+Lemma upd_complete : forall l x MAX, (length l < MAX)%nat -> 
+  upd_Znth (Zlength l) (complete MAX l) x = complete MAX (l ++ [x]).
+Proof.
+  intros; unfold complete.
+  rewrite upd_Znth_app2, Zminus_diag.
+  rewrite app_length; simpl plus.
+  destruct (MAX - length l)%nat eqn: Hminus; [omega|].
+  replace (MAX - (length l + 1))%nat with n by omega.
+  unfold upd_Znth, sublist.sublist; simpl.
+  rewrite Zlength_cons.
+  unfold Z.succ; rewrite Z.add_simpl_r.
+  rewrite Zlength_correct, Nat2Z.id, firstn_exact_length.
+  rewrite <- app_assoc; auto.
+  { repeat rewrite Zlength_correct; omega. }
+Qed.
+
+Lemma Znth_complete : forall n l d MAX, n < Zlength l -> Znth n (complete MAX l) d = Znth n l d.
+Proof.
+  intros; apply app_Znth1; auto.
+Qed.
+
+Lemma remove_complete : forall l x MAX, (length l < MAX)%nat -> 
+  upd_Znth (Zlength l) (complete MAX (l ++ [x])) (Vint (Int.repr 0)) = complete MAX l.
+Proof.
+  intros; unfold complete.
+  rewrite upd_Znth_app1; [|repeat rewrite Zlength_correct; rewrite app_length; simpl; Omega0].
+  rewrite app_length; simpl plus.
+  rewrite upd_Znth_app2, Zminus_diag; [|rewrite Zlength_cons; simpl; omega].
+  unfold upd_Znth, sublist.sublist.
+  rewrite Zminus_diag; simpl firstn.
+  destruct (MAX - length l)%nat eqn: Hminus; [omega|].
+  replace (MAX - (length l + 1))%nat with n by omega.
+  simpl.
+  rewrite <- app_assoc; auto.
+Qed.
+
+Lemma Forall_app : forall A (P : A -> Prop) l1 l2,
+  Forall P (l1 ++ l2) <-> Forall P l1 /\ Forall P l2.
+Proof.
+  induction l1; split; auto; intros.
+  - destruct H; auto.
+  - inversion H as [|??? H']; subst.
+    rewrite IHl1 in H'; destruct H'; split; auto.
+  - destruct H as (H & ?); inv H; constructor; auto.
+    rewrite IHl1; split; auto.
+Qed.
+
+Lemma repeat_plus : forall A (x : A) i j, repeat x (i + j) = repeat x i ++ repeat x j.
+Proof.
+  induction i; auto; simpl; intro.
+  rewrite IHi; auto.
+Qed.
+
+Definition remove_at {A} i (l : list A) := firstn i l ++ skipn (S i) l.
+
+Lemma upd_Znth_cons : forall {A} i a l (x : A), i > 0 ->
+  upd_Znth i (a :: l) x = a :: upd_Znth (i - 1) l x.
+Proof.
+  intros; unfold upd_Znth, sublist.sublist; simpl.
+  repeat rewrite Z.sub_0_r.
+  destruct (Z.to_nat i) eqn: Hi.
+  { exploit Z2Nat_inj_0; eauto; omega. }
+  rewrite Zlength_cons; repeat rewrite Z2Nat.inj_add; try omega.
+  repeat rewrite Z2Nat.inj_sub; try omega.
+  rewrite Hi; simpl.
+  rewrite Nat.sub_0_r.
+  do 4 f_equal.
+  rewrite Z2Nat.inj_succ; [|rewrite Zlength_correct; omega].
+  repeat rewrite Z2Nat.inj_add; try omega.
+  rewrite Z2Nat.inj_sub; try omega.
+  simpl plus; omega.
+Qed.
+
+Lemma Forall_firstn : forall {A} (P : A -> Prop) l i, Forall P l ->
+  Forall P (firstn i l).
+Proof.
+  intros; rewrite Forall_forall in *.
+  intros ? Hin; pose proof (firstn_In _ _ _ Hin); auto.
+Qed.
+
+Lemma Forall_skipn : forall {A} (P : A -> Prop) l i, Forall P l ->
+  Forall P (skipn i l).
+Proof.
+  intros; rewrite Forall_forall in *.
+  intros ? Hin; pose proof (skipn_In _ _ _ Hin); auto.
+Qed.
+
+Lemma Forall_sublist : forall {A} (P : A -> Prop) l i j, Forall P l ->
+  Forall P (sublist.sublist i j l).
+Proof.
+  intros; unfold sublist.sublist.
+  apply Forall_firstn; apply Forall_skipn; auto.
+Qed.
+
+Lemma Forall_upd_Znth : forall {A} (P : A -> Prop) x l i, Forall P l -> P x ->
+  Forall P (upd_Znth i l x).
+Proof.
+  intros; unfold upd_Znth.
+  rewrite Forall_app; split; [|constructor; auto]; apply Forall_sublist; auto.
+Qed.
+
+Lemma last_cons : forall {A} (d : A) l x, l <> [] -> last (x :: l) d = last l d.
+Proof.
+  intros.
+  destruct l; auto.
+  contradiction H; auto.
+Qed.
+
+Lemma nth_last : forall {A} (d : A) l, nth (length l - 1) l d = last l d.
+Proof.
+  induction l; auto.
+  simpl nth.
+  destruct (length l) eqn: Hlen.
+  { destruct l; simpl in *; [auto | omega]. }
+  rewrite last_cons; simpl in *; [|intro; subst; discriminate].
+  rewrite NPeano.Nat.sub_0_r in IHl; auto.
+Qed.
+
+Lemma Znth_last : forall {A} l (d : A), Znth (Zlength l - 1) l d = last l d.
+Proof.
+  intros; unfold Znth.
+  destruct (zlt (Zlength l - 1) 0).
+  - destruct l; auto.
+    rewrite Zlength_correct in *; simpl length in *.
+    rewrite Nat2Z.inj_succ in *; omega.
+  - rewrite Z2Nat.inj_sub; [|omega].
+    rewrite Zlength_correct, Nat2Z.id; simpl.
+    apply nth_last.
+Qed.
+
+Lemma sepcon_app : forall l1 l2, fold_right sepcon emp (l1 ++ l2) =
+  fold_right sepcon emp l1 * fold_right sepcon emp l2.
+Proof.
+  induction l1; simpl; intros.
+  - rewrite emp_sepcon; auto.
+  - rewrite IHl1, sepcon_assoc; auto.
+Qed.
+
+(*Lemma lock_precise : forall {cs} sh b o, readable_share sh -> precise (@data_at_ cs sh tlock (Vptr b o)).
+Proof.
+  intros.
+  unfold data_at_, field_at_, field_at, at_offset; simpl.
+  apply precise_andp2.
+  rewrite data_at_rec_eq; unfold withspacer, at_offset; simpl.
+  unfold tlock, default_val; simpl.
+  unfold reptype_gen.
+  simpl.
+  
+Print reptype_gen.
+Print default_val.
+  rewrite data_at_rec_eq; unfold withspacer, at_offset; simpl.
+  rewrite data_at_rec_eq; unfold withspacer, at_offset; simpl.
+  unfold array_pred, aggregate_pred.array_pred; simpl.
+  unfold Zlength, Znth; simpl.
+  rewrite data_at_rec_eq; simpl.
+  rewrite data_at_rec_eq; simpl.
+  apply precise_sepcon; apply precise_andp2; repeat apply precise_sepcon; try apply precise_emp;
+    apply mapsto_undef_precise; auto.
+Qed.
+
+*)
